@prefix dc: <http://purl.org/dc/elements/1.1/> .
@prefix grddl: <http://www.w3.org/2003/g/data-view#> .
@prefix owl: <http://www.w3.org/2002/07/owl#> .
@prefix rdf: <http://www.w3.org/1999/02/22-rdf-syntax-ns#> .
@prefix rdfs: <http://www.w3.org/2000/01/rdf-schema#> .
@prefix xml: <http://www.w3.org/XML/1998/namespace> .
@prefix xsd: <http://www.w3.org/2001/XMLSchema#> .
@prefix plowl: <http://niche.cs.dal.ca/2017/06/plowl#> .

<http://niche.cs.dal.ca/2017/06/plowl/> a owl:Ontology ;
     dc:title "Plausible OWL Schema vocabulary" ;
     rdfs:comment """
		This ontology partially describes the plausible extensions to OWL. This extension includes
		classes and properties that together form the basis of the PL-OWL.
		""" ;
     rdfs:isDefinedBy
          <http://www.w3.org/TR/owl2-mapping-to-rdf/>,
          <http://www.w3.org/TR/owl2-rdf-based-semantics/>,
          <http://www.w3.org/TR/owl2-syntax/> ;
     rdfs:seeAlso   <http://www.w3.org/TR/owl2-rdf-based-semantics/#table-axiomatic-classes>,
                    <http://www.w3.org/TR/owl2-rdf-based-semantics/#table-axiomatic-properties> ;
     owl:imports <http://www.w3.org/2000/01/rdf-schema>,
					<http://www.w3.org/2002/07/owl> ;
     owl:versionIRI <http://niche.cs.dal.ca/2017/06/plowl> ;
     owl:versionInfo "$Date: 2016/11/07 14:59:12 $" ;
     grddl:namespaceTransformation <http://dev.w3.org/cvsweb/2009/owl-grddl/owx2rdf.xsl> .  


 
plowl:OrderedProperty 
	a owl:Class ;
    	 rdfs:label "OrderedProperty" ;
     	 rdfs:comment "The class of ordered properties." ;
    	 rdfs:isDefinedBy <http://niche.cs.dal.ca/2017/06/plowl#> ;
    	 rdfs:subClassOf owl:ObjectProperty. 
	 

plowl:Context 
	a owl:Class;
	 rdfs:subClassOf rdf:Node;
	 rdfs:label "Context" ;
    	 rdfs:comment "Represents the context of the object property." ;
     	 rdfs:isDefinedBy <http://niche.cs.dal.ca/2017/06/plowl#> .
	 
plowl:PlausiblePattern 
	a owl:Class;
	 rdfs:subClassOf rdf:Node;
	 rdfs:label "Plausible Pattern" ;
    	 rdfs:comment "Collection of the plausible patterns." ;
     	rdfs:isDefinedBy <http://niche.cs.dal.ca/2017/06/plowl#> .

plowl:PlausibleAnswer 
	a owl:Class;
	 rdfs:label "Plausible Answer" ;
    	 rdfs:comment "Represent the plasubily inferred triples." ;
    	 rdfs:isDefinedBy <http://niche.cs.dal.ca/2017/06/plowl#>;
	 rdfs:subClassOf [
		a owl:Restriction ;
		owl:onProperty plowl:inferredThroughPattern ;
		owl:allValuesFrom [
			a owl:Class ;
			owl:unionOf (
				<http://web.cs.dal.ca/~hossein/plowl/univ-bench.owl#Generalization>
				<http://web.cs.dal.ca/~hossein/plowl/univ-bench.owl#Specialization>
				<http://web.cs.dal.ca/~hossein/plowl/univ-bench.owl#Similarity>
				<http://web.cs.dal.ca/~hossein/plowl/univ-bench.owl#Dissimilarity>
				<http://web.cs.dal.ca/~hossein/plowl/univ-bench.owl#Afortiori>
				<http://web.cs.dal.ca/~hossein/plowl/univ-bench.owl#Interpolation>
			)
			]
		],
		[
		a owl:Restriction ;
		owl:onProperty plowl:inTheContextOf ;
		owl:someValuesFrom plowl:Context
		];
	 
plowl:hasContext 
	a owl:ObjectProperty;	  
	  rdfs:range plowl:Context;
	  rdfs:comment "This object property links an opject property to the context nodes being applied to it."^^xsd:string ;
	  rdfs:isDefinedBy <http://niche.cs.dal.ca/2017/06/plowl#> .

plowl:standsAfter 
	a owl:OrderedProperty;	  
	  rdfs:range owl:Thing;
	  rdfs:domain owl:Thing;
	  rdfs:comment "This object property is used to model ordering relation to show which concept (subject) locates after another concept (object) regarding a specific context. The inverse property is standsBefore.."^^xsd:string ;
	  rdfs:isDefinedBy <http://niche.cs.dal.ca/2017/06/plowl#> .	  
	 
plowl:standsBefore 
	a owl:OrderedProperty;	  
	  rdfs:range owl:Thing;
	  rdfs:domain owl:Thing;
	  rdfs:comment "This object property is used to model ordering relation to show which concept (subject) locates before another concept (object) regarding a specific context. The inverse property is standsAfter.."^^xsd:string ;
	  rdfs:isDefinedBy <http://niche.cs.dal.ca/2017/06/plowl#> .	
	  
plowl:hasSubject 			
	a owl:ObjectProperty;	  
	  rdfs:domain plowl:PlausibleAnswer;
	  rdfs:range  owl:Thing;
	  rdfs:comment "This object property links a plausible answer to its subject."^^xsd:string ;
	  rdfs:isDefinedBy <http://niche.cs.dal.ca/2017/06/plowl#> .

plowl:hasObject 			
	a owl:ObjectProperty;	  
	  rdfs:domain plowl:PlausibleAnswer;
	  rdfs:range  owl:Thing;
	  rdfs:comment "This object property links a plausible answer to its object."^^xsd:string ;
	  rdfs:isDefinedBy <http://niche.cs.dal.ca/2017/06/plowl#> .	  
	  
plowl:hasPredicate 			
	a owl:ObjectProperty;	  
	  rdfs:domain plowl:PlausibleAnswer;
	  rdfs:range  owl:Thing;
	  rdfs:comment "This object property links a plausible answer to its predicate."^^xsd:string ;
	  rdfs:isDefinedBy <http://niche.cs.dal.ca/2017/06/plowl#> .
	  
plwol:inferredThroughPattern 
	a owl:ObjectProperty;	  
	  rdfs:domain plowl:PlausibleAnswer;
	  rdfs:range  owl:PlausiblePattern;
	  rdfs:comment "This object property links a plausible answer to the plausible pattern that lead to the inference."^^xsd:string ;
	  rdfs:isDefinedBy <http://niche.cs.dal.ca/2017/06/plowl#> .	
		
plwol:inTheContextOf 
	a owl:ObjectProperty;	  
	  rdfs:domain plowl:PlausibleAnswer;
	  rdfs:range  plowl:Context;
	  rdfs:comment "This object property links a plausible answer to the context that lead to the inference."^^xsd:string ;
	  rdfs:isDefinedBy <http://niche.cs.dal.ca/2017/06/plowl#> .